proof/refine/ARM/CSpace1_R.thy
@@ -1830,7 +1830,7 @@ lemma descendants_of_eq':
 \<comment>\<open>
   This turned out to be the least-annoying way to deal with
   the subgoal @{term
-    "ps' |> reply_of' |> replyNext = replyNexts_of s'"
+    "ps' |> reply_of' |> replyNext_of = replyNexts_of s'"
   } which shows up in the proof of `cap_update_corres`.
 
   `ps'` here comes from `ksPSpace s''`, where `s''` is the new state
